WebAssembly/Wasm_Properties_Aux.thy
@@ -395,7 +395,7 @@ lemma b_e_type_return_call:
   assumes "\<C> \<turnstile> [e] : (ts _> ts')"
           "e = ReturnCall i"
   shows  "i < length (func_t \<C>)"
-         "\<exists>ts'' tf1 tf2. ts = ts''@tf1 \<and> ts' = ts''@tf2 \<and> (func_t \<C>)!i = (tf1 _> tf2)"
+         "\<exists>ts'' tf1 tf2. ts = ts''@tf1 \<and> (func_t \<C>)!i = (tf1 _> tf2) \<and> (return \<C>) = Some tf2"
   using assms
   by (induction "[e]" "(ts _> ts')" arbitrary: ts ts' rule: b_e_typing.induct, auto)
 
@@ -403,7 +403,7 @@ lemma b_e_type_return_call_indirect:
   assumes "\<C> \<turnstile> [e] : (ts _> ts')"
           "e = ReturnCall_indirect i"
   shows "i < length (types_t \<C>)"
-        "\<exists>ts'' tf1 tf2. ts = ts''@tf1@[T_i32] \<and> ts' = ts''@tf2 \<and> (types_t \<C>)!i = (tf1 _> tf2)"
+        "\<exists>ts'' tf1 tf2. ts = ts''@tf1@[T_i32] \<and> (types_t \<C>)!i = (tf1 _> tf2) \<and> (return \<C>) = Some tf2"
   using assms
   by (induction "[e]" "(ts _> ts')" arbitrary: ts ts' rule: b_e_typing.induct, auto)
 
